@prefix semts:        <https://w3id.org/semts/ontology#> .
@prefix owl:          <http://www.w3.org/2002/07/owl#> .
@prefix rdf:          <http://www.w3.org/1999/02/22-rdf-syntax-ns#> .
@prefix xml:          <http://www.w3.org/XML/1998/namespace> .
@prefix xsd:          <http://www.w3.org/2001/XMLSchema#> .
@prefix rdfs:         <http://www.w3.org/2000/01/rdf-schema#> .
@prefix skos:         <http://www.w3.org/2004/02/skos/core#> .
@prefix time:         <http://www.w3.org/2006/time#> .
@prefix vann:         <http://purl.org/vocab/vann/> .
@prefix dcterms:      <http://purl.org/dc/terms/> .
@prefix mls:          <http://www.w3.org/ns/mls#> .
@prefix dcat:         <http://www.w3.org/ns/dcat#> .
@prefix prov:         <http://www.w3.org/ns/prov#> .

semts:
    rdf:type                      owl:Ontology ;
    owl:imports                   <http://w3id.org/mlso> ;

    # Basic Metadata
    rdfs:label                    "Time Series Knowledge (SemTS) Ontology"@en ;
    rdfs:comment                  "An Ontology for the Semantic Categorization of Time Series Knowledge."@en ;

    # Version Information
    owl:versionInfo               "0.1.0"^^xsd:string ;     # Using Semantic Versioning 2.0 Format: Major.Minor.Patch

    # Namespace Information
    vann:preferredNamespacePrefix "semts" ;
    vann:preferredNamespaceUri    "https://w3id.org/semts/ontology#" ;

    # Additional Metadata
    dcterms:subject               "Time Series"@en, "Data Analytics"@en, "Knowledge Graph"@en ;
    dcterms:creator               "Alexander Gra√ü" .
.

#################################################################
#    Object Properties
#################################################################

###  https://w3id.org/semts/ontology#dataReferenceIndex
semts:dataReferenceIndex
    rdf:type     owl:ObjectProperty ;
    rdfs:domain  semts:RawDataReference ;
    rdfs:range   semts:TimeIndex ;
    rdfs:label   "Data Reference Index"@en ;
    rdfs:comment "Index associated with the raw data of a segment descriptor"@en .


###  https://w3id.org/semts/ontology#dataReferenceSource
semts:dataReferenceSource
    rdf:type     owl:ObjectProperty ;
    rdfs:domain  semts:RawDataReference ;
    rdfs:range   dcat:Resource ;
    rdfs:label   "Data Reference Source"@en ;
    rdfs:comment "Data source associated with the raw data of a segment descriptor"@en .


###  https://w3id.org/semts/ontology#dataReferenceStructure
semts:dataReferenceStructure
    rdf:type     owl:ObjectProperty ;
    rdfs:domain  semts:RawDataReference ;
    rdfs:range   semts:DataStructure ;
    rdfs:label   "Data Reference Structure"@en ;
    rdfs:comment "Set of dimensions associated with the raw data of a segment descriptor"@en .


###  https://w3id.org/semts/ontology#dataStructure
semts:dataStructure
    rdf:type     owl:ObjectProperty ;
    rdfs:domain  semts:SegmentDescriptor ;
    rdfs:range   semts:DataStructure ;
    rdfs:label   "Data Structure"@en ;
    rdfs:comment "Set of dimensions associated with a segment descriptor"@en .


###  https://w3id.org/semts/ontology#generationInputKnowledge
semts:generationInputKnowledge
    rdf:type     owl:ObjectProperty ;
    rdfs:domain  semts:KnowledgeGenerationEntity ;
    rdfs:range   semts:Knowledge ;
    rdfs:label   "Generation Input Knowledge"@en ;
    rdfs:comment "Knowledge that is used to derive further knowledge via knowledge generation"@en .


###  https://w3id.org/semts/ontology#generationMethodRun
semts:generationMethodRun
    rdf:type     owl:ObjectProperty ;
    rdfs:domain  semts:KnowledgeGenerationMethod ;
    rdfs:range   mls:Run ;
    rdfs:label   "Generation Method Run"@en ;
    rdfs:comment "Connection to metadata describing specific information of the knowledge generation process"@en .


###  https://w3id.org/semts/ontology#groupKnowledge
semts:groupKnowledge
    rdf:type     owl:ObjectProperty ;
    rdfs:domain  semts:KnowledgeGroup, semts:SegmentDescriptorGroup ;
    rdfs:range   semts:Knowledge ;
    rdfs:label   "Group Knowledge"@en ;
    rdfs:comment "Knowledge belonging to a group of semantically connected instances"@en .


###  https://w3id.org/semts/ontology#groupSegments
semts:groupSegments
    rdf:type     owl:ObjectProperty ;
    rdfs:domain  semts:SegmentDescriptorGroup ;
    rdfs:range   semts:SegmentDescriptor ;
    rdfs:label   "Group Segments"@en ;
    rdfs:comment "Segments belonging to a group in order to create segment collections"@en .


###  https://w3id.org/semts/ontology#knowledgeConcept
semts:knowledgeConcept
    rdf:type     owl:ObjectProperty ;
    rdfs:domain  semts:Knowledge ;
    rdfs:range   semts:KnowledgeConcept ;
    rdfs:label   "Knowledge Concept"@en ;
    rdfs:comment "The concept to semantically structure time series knowledge"@en .


###  https://w3id.org/semts/ontology#knowledgeGenerationEntity
semts:knowledgeGenerationEntity
    rdf:type     owl:ObjectProperty, owl:FunctionalProperty ;
    rdfs:domain  semts:Knowledge ;
    rdfs:range   semts:KnowledgeGenerationEntity ;
    rdfs:label   "Knowledge Generation Entity"@en ;
    rdfs:comment "The generation entity, which led to the creation of particular knowledge instances"@en .


###  https://w3id.org/semts/ontology#knowledgeOrigin
semts:knowledgeOrigin
    rdf:type     owl:ObjectProperty ;
    rdfs:domain  semts:MethodKnowledge, semts:ScenarioKnowledge ;
    rdfs:range   prov:Agent ;
    rdfs:label   "Knowledge Origin"@en ;
    rdfs:comment "The traceable origin of generated knowledge"@en .


###  https://w3id.org/semts/ontology#knowledgeQualityMeasure
semts:knowledgeQualityMeasure
    rdf:type     owl:ObjectProperty ;
    rdfs:domain  semts:Knowledge ;
    rdfs:range   semts:KnowledgeQualityMeasure ;
    rdfs:label   "Knowledge Quality Measure"@en ;
    rdfs:comment "The quality measure associated with a knowledge instance"@en .


###  https://w3id.org/semts/ontology#mathFieldConcept
semts:mathFieldConcept
    rdf:type     owl:ObjectProperty ;
    rdfs:domain  semts:MathExpression ;
    rdfs:range   semts:MathFieldConcept ;
    rdfs:label   "Math Field Concept"@en ;
    rdfs:comment "The mathematical field associated with a mathematical expressions"@en .


###  https://w3id.org/semts/ontology#presetMethod
semts:presetMethod
    rdf:type     owl:ObjectProperty ;
    rdfs:domain  semts:MethodKnowledge ;
    rdfs:range   mls:Algorithm ;
    rdfs:label   "Preset Method"@en ;
    rdfs:comment "A particular algorithm that was used for the generation of knowledge"@en .


###  https://w3id.org/semts/ontology#presetParameters
semts:presetParameters
    rdf:type     owl:ObjectProperty ;
    rdfs:domain  semts:MethodKnowledge ;
    rdfs:range   mls:HyperParameterSetting ;
    rdfs:label   "Preset Parameters"@en ;
    rdfs:comment "A particular hyperparameter setting that was used for the generation of knowledge"@en .


###  https://w3id.org/semts/ontology#qualityMeasureConcept
semts:qualityMeasureConcept
    rdf:type     owl:ObjectProperty ;
    rdfs:domain  semts:KnowledgeQualityMeasure ;
    rdfs:range   semts:QualityMeasureConcept ;
    rdfs:label   "Quality Measure Concept"@en ;
    rdfs:comment "Concept describing the used quality measure during knowledge generation"@en .


###  https://w3id.org/semts/ontology#segmentIndex
semts:segmentIndex
    rdf:type     owl:ObjectProperty ;
    rdfs:domain  semts:SegmentDescriptor ;
    rdfs:range   semts:TimeIndex ;
    rdfs:label   "Segment Index"@en ;
    rdfs:comment "Index associated with a segment descriptor"@en .


###  https://w3id.org/semts/ontology#segmentKnowledge
semts:segmentKnowledge
    rdf:type     owl:ObjectProperty ;
    rdfs:domain  semts:SegmentDescriptor ;
    rdfs:range   semts:Knowledge ;
    rdfs:label   "Segment Knowledge"@en ;
    rdfs:comment "Knowledge associated with a segment descriptor"@en .


###  https://w3id.org/semts/ontology#segmentSeries
semts:segmentSeries
    rdf:type     owl:ObjectProperty ;
    rdfs:domain  semts:SegmentDescriptor ;
    rdfs:range   semts:SeriesData ;
    rdfs:label   "Segment Series"@en ;
    rdfs:comment "Series associated with a segment descriptor"@en .


###  https://w3id.org/semts/ontology#seriesComponentType
semts:seriesComponentType
    rdf:type     owl:ObjectProperty, owl:FunctionalProperty ;
    rdfs:domain  semts:SeriesComponentGroup, semts:SeriesComponentProperty ;
    rdfs:range   semts:DispersionComponentConcept, semts:LocationComponentConcept, semts:StructuralComponentConcept,
                 semts:TrendComponentConcept ;
    rdfs:label   "Series Component Type"@en ;
    rdfs:comment "Concept to define the type of time series knowledge. Each type can be of: Dispersion, Location, Trend or Structural"@en .


###  https://w3id.org/semts/ontology#structureDimension
semts:structureDimension
    rdf:type     owl:ObjectProperty ;
    rdfs:domain  semts:DataStructure ;
    rdfs:range   semts:SeriesDimension ;
    rdfs:label   "Structure Dimension"@en ;
    rdfs:comment "Dimensions belonging to a data set. This can be the set of dimensions describing a multivariate time series"@en .


#################################################################
#    Data properties
#################################################################

###  https://w3id.org/semts/ontology#dimensionPosition
semts:dimensionPosition
    rdf:type     owl:DatatypeProperty ;
    rdfs:domain  semts:SeriesDimension ;
    rdfs:range   xsd:integer ;
    rdfs:label   "Dimension Position"@en ;
    rdfs:comment "Index position of a dimension in an ordered set of dimensions (e.g. index position in a dataframe)"@en .


###  https://w3id.org/semts/ontology#dimensionUnit
semts:dimensionUnit
    rdf:type     owl:DatatypeProperty ;
    rdfs:domain  semts:SeriesDimension ;
    rdfs:range   xsd:string ;
    rdfs:label   "Dimension Unit"@en ;
    rdfs:comment "Unit of the data"@en .

# todo: why not reuse rdfs:comment or dcterms:description instead?
###  https://w3id.org/semts/ontology#hasDescription
semts:hasDescription
    rdf:type     owl:DatatypeProperty ;
    rdfs:domain  semts:Knowledge, semts:KnowledgeGenerationEntity, semts:KnowledgeQualityMeasure,
                 semts:SeriesDimension ;
    rdfs:range   xsd:string ;
    rdfs:label   "Has Description"@en ;
    rdfs:comment "Description property associated with multiple classes"@en .

###  https://w3id.org/semts/ontology#hasDtype
semts:hasDtype
    rdf:type     owl:DatatypeProperty ;
    rdfs:domain  semts:KnowledgeQualityMeasure, semts:ScenarioParameter, semts:SegmentProperty, semts:SeriesDimension ;
    rdfs:range   xsd:string ;
    rdfs:label   "Has Data Type"@en ;
    rdfs:comment "Data type of linked values"@en .

# todo: why not reuse rdfs:label or dcterms:title instead?
###  https://w3id.org/semts/ontology#hasName
semts:hasName
    rdf:type     owl:DatatypeProperty ;
    rdfs:domain  semts:Knowledge, semts:KnowledgeGenerationEntity, semts:KnowledgeQualityMeasure,
                 semts:SeriesDimension ;
    rdfs:range   xsd:string ;
    rdfs:label   "Has Name"@en ;
    rdfs:comment "Name of a specific instance"@en .


###  https://w3id.org/semts/ontology#hasValue
semts:hasValue
    rdf:type     owl:DatatypeProperty ;
    rdfs:domain  semts:KnowledgeQualityMeasure, semts:Label, semts:MathExpression, semts:Note, semts:ScenarioParameter,
                 semts:SegmentProperty ;
    rdfs:range   xsd:string ;
    rdfs:label   "Has Value"@en ;
    rdfs:comment "Value associated with multiple classes such as different knowledge classes"@en .


###  https://w3id.org/semts/ontology#mathExpressionFormat
semts:mathExpressionFormat
    rdf:type     owl:DatatypeProperty ;
    rdfs:domain  semts:MathExpression ;
    rdfs:range   xsd:string ;
    rdfs:label   "Math Expression Format"@en ;
    rdfs:comment "The format of a defined math expression"@en .


###  https://w3id.org/semts/ontology#mathExpressionParser
semts:mathExpressionParser
    rdf:type     owl:DatatypeProperty ;
    rdfs:domain  semts:MathExpression ;
    rdfs:range   xsd:string ;
    rdfs:label   "Math Expression Parser"@en ;
    rdfs:comment "A translator or parser to evaluate the syntax of mathematical expressions"@en .


#################################################################
#    Classes
#################################################################

###  http://www.w3.org/2004/02/skos/core#Concept
skos:Concept
    rdf:type owl:Class .


###  http://www.w3.org/2006/time#TemporalEntity
time:TemporalEntity
    rdf:type owl:Class .


###  http://www.w3.org/ns/dcat#Resource
dcat:Resource
    rdf:type owl:Class .


###  http://www.w3.org/ns/mls#Algorithm
mls:Algorithm
    rdf:type owl:Class .


###  http://www.w3.org/ns/mls#Dataset
mls:Dataset
    rdf:type owl:Class .


###  http://www.w3.org/ns/mls#Feature
mls:Feature
    rdf:type owl:Class .


###  http://www.w3.org/ns/mls#HyperParameterSetting
mls:HyperParameterSetting
    rdf:type owl:Class .


###  http://www.w3.org/ns/mls#Run
mls:Run
    rdf:type owl:Class .


###  http://www.w3.org/ns/prov#Agent
prov:Agent
    rdf:type owl:Class .


###  https://w3id.org/semts/ontology#Condition
semts:Condition
    rdf:type        owl:Class ;
    rdfs:subClassOf semts:MathExpression ;
    rdfs:label      "Condition"@en ;
    rdfs:comment    "Knowledge to describe a conditional statement"@en .


###  https://w3id.org/semts/ontology#DataInformationProperty
semts:DataInformationProperty
    rdf:type        owl:Class ;
    rdfs:subClassOf semts:SegmentProperty ;
    rdfs:label      "Data Information Property"@en ;
    rdfs:comment    "Knowledge to describe general information associated with the time series such as the number of missing points"@en .


###  https://w3id.org/semts/ontology#DataKnowledge
semts:DataKnowledge
    rdf:type        owl:Class ;
    rdfs:subClassOf semts:Knowledge ;
    rdfs:label      "Data Knowledge"@en ;
    rdfs:comment    "Defines knowledge derived from the time series data"@en .


###  https://w3id.org/semts/ontology#DataStructure
semts:DataStructure
    rdf:type        owl:Class ;
    rdfs:subClassOf owl:Thing ;
    rdfs:label      "Data Structure"@en ;
    rdfs:comment    "Definition of the data structure of a time series segment. Especially defines the set of dimensions"@en .


###  https://w3id.org/semts/ontology#DispersionComponentConcept
semts:DispersionComponentConcept
    rdf:type        owl:Class ;
    rdfs:subClassOf skos:Concept ;
    rdfs:label      "Dispersion Component Concept"@en ;
    rdfs:comment    "Concept to describe knowledge of type dispersion"@en .


###  https://w3id.org/semts/ontology#Knowledge
semts:Knowledge
    rdf:type        owl:Class ;
    rdfs:subClassOf owl:Thing ;
    rdfs:label      "Knowledge"@en ;
    rdfs:comment    "Most generic class to define knowledge entities"@en .


###  https://w3id.org/semts/ontology#KnowledgeConcept
semts:KnowledgeConcept
    rdf:type        owl:Class ;
    rdfs:subClassOf skos:Concept ;
    rdfs:label      "Knowledge Concept"@en ;
    rdfs:comment    "Parental class of all knowledge concepts"@en .


###  https://w3id.org/semts/ontology#KnowledgeDissimilarityMeasure
semts:KnowledgeDissimilarityMeasure
    rdf:type        owl:Class ;
    rdfs:subClassOf semts:KnowledgeGenerationEntity ;
    rdfs:label      "Knowledge Dissimilarity Measure"@en ;
    rdfs:comment    "Defines a similarity measure applied to knowledge in order to derive further knowledge"@en .


###  https://w3id.org/semts/ontology#KnowledgeGenerationEntity
semts:KnowledgeGenerationEntity
    rdf:type     owl:Class ;
    rdfs:label   "Knowledge Generation Entity"@en ;
    rdfs:comment "Most generic class to define knowledge generation instances"@en .


###  https://w3id.org/semts/ontology#KnowledgeGenerationMethod
semts:KnowledgeGenerationMethod
    rdf:type        owl:Class ;
    rdfs:subClassOf mls:Algorithm, semts:KnowledgeGenerationEntity ;
    rdfs:label      "Knowledge Generation Method"@en ;
    rdfs:comment    "Defines knowledge that was produced by a method"@en .


###  https://w3id.org/semts/ontology#KnowledgeGroup
semts:KnowledgeGroup
    rdf:type        owl:Class ;
    rdfs:subClassOf semts:Knowledge ;
    rdfs:label      "Knowledge Group"@en ;
    rdfs:comment    "Group to allow for knowledge hierarchies or to cluster semantically aligned knowledge"@en .


###  https://w3id.org/semts/ontology#KnowledgeQualityMeasure
semts:KnowledgeQualityMeasure
    rdf:type        owl:Class ;
    rdfs:subClassOf owl:Thing ;
    rdfs:label      "Knowledge Quality Measure"@en ;
    rdfs:comment    "A measure to define the goodness of knowledge"@en .


###  https://w3id.org/semts/ontology#KnowledgeReasoning
semts:KnowledgeReasoning
    rdf:type        owl:Class ;
    rdfs:subClassOf semts:KnowledgeGenerationEntity ;
    rdfs:label      "Knowledge Reasoning"@en ;
    rdfs:comment    "Defines the generation of knowledge that was derived via a semantic reasoning"@en .


###  https://w3id.org/semts/ontology#Label
semts:Label
    rdf:type        owl:Class ;
    rdfs:subClassOf semts:ScenarioKnowledge ;
    rdfs:label      "Label"@en ;
    rdfs:comment    "Defines knowledge which is linked to a specific scenario rather than the data itself. For instance knowledge from domain experts"@en .


###  https://w3id.org/semts/ontology#LocationComponentConcept
semts:LocationComponentConcept
    rdf:type        owl:Class ;
    rdfs:subClassOf skos:Concept ;
    rdfs:label      "Location Component Concept"@en ;
    rdfs:comment    "Concept to describe knowledge of type location"@en .


###  https://w3id.org/semts/ontology#MathExpression
semts:MathExpression
    rdf:type        owl:Class ;
    rdfs:subClassOf semts:ScenarioKnowledge ;
    rdfs:label      "Math Expression"@en ;
    rdfs:comment    "Knowledge defining mathematical expressions"@en .


###  https://w3id.org/semts/ontology#MathFieldConcept
semts:MathFieldConcept
    rdf:type        owl:Class ;
    rdfs:subClassOf skos:Concept ;
    rdfs:label      "Math Field Concept"@en ;
    rdfs:comment    "Concepts to semantically structure mathematical knowledge"@en .


###  https://w3id.org/semts/ontology#MethodKnowledge
semts:MethodKnowledge
    rdf:type        owl:Class ;
    rdfs:subClassOf semts:Knowledge ;
    rdfs:label      "Method Knowledge"@en ;
    rdfs:comment    "Knowledge that defines methodical presets"@en .


###  https://w3id.org/semts/ontology#Note
semts:Note
    rdf:type        owl:Class ;
    rdfs:subClassOf semts:ScenarioKnowledge ;
    rdfs:label      "Note"@en ;
    rdfs:comment    "Knowledge to classify purely textual annotations"@en .


###  https://w3id.org/semts/ontology#PredictionProperty
semts:PredictionProperty
    rdf:type        owl:Class ;
    rdfs:subClassOf semts:SegmentProperty ;
    rdfs:label      "Prediction Property"@en ;
    rdfs:comment    "Knowledge to define resultant predictions from an exploitation of other knowledge"@en .


###  https://w3id.org/semts/ontology#QualityMeasureConcept
semts:QualityMeasureConcept
    rdf:type        owl:Class ;
    rdfs:subClassOf skos:Concept ;
    rdfs:label      "Quality Measure Concept"@en ;
    rdfs:comment    "Concept to specify the category of a knowledge quality measure"@en .


###  https://w3id.org/semts/ontology#RawDataReference
semts:RawDataReference
    rdf:type        owl:Class ;
    rdfs:subClassOf semts:DataKnowledge ;
    rdfs:label      "Raw Data Reference"@en ;
    rdfs:comment    "Reference to concrete data which is considered the most complete yet unprocessed type of knowledge"@en .


###  https://w3id.org/semts/ontology#RootSegmentDescriptor
semts:RootSegmentDescriptor
    rdf:type        owl:Class ;
    rdfs:subClassOf semts:SegmentDescriptor ;
    rdfs:label      "Root Segment Descriptor"@en ;
    rdfs:comment    "A class to link all the information associated with a complete time series. The interface between data information and associated or generated knowledge"@en .


###  https://w3id.org/semts/ontology#ScenarioKnowledge
semts:ScenarioKnowledge
    rdf:type        owl:Class ;
    rdfs:subClassOf semts:Knowledge ;
    rdfs:label      "Scenario Knowledge"@en ;
    rdfs:comment    "todo: update"@en .


###  https://w3id.org/semts/ontology#ScenarioParameter
semts:ScenarioParameter
    rdf:type        owl:Class ;
    rdfs:subClassOf semts:ScenarioKnowledge ;
    rdfs:label      "Scenario Parameter"@en ;
    rdfs:comment    "todo: update"@en .


###  https://w3id.org/semts/ontology#SegmentDescriptor
semts:SegmentDescriptor
    rdf:type        owl:Class ;
    rdfs:subClassOf owl:Thing ;
    rdfs:label      "Segment Descriptor"@en ;
    rdfs:comment    "A class to link all the information associated with a partial time series regarding dimensionality or index interval. The interface between data information and associated or generated knowledge"@en .


###  https://w3id.org/semts/ontology#SegmentDescriptorGroup
semts:SegmentDescriptorGroup
    rdf:type     owl:Class ;
    rdfs:label   "Segment Descriptor Group"@en ;
    rdfs:comment "A group to define segment descriptor collections"@en .


###  https://w3id.org/semts/ontology#SegmentProperty
semts:SegmentProperty
    rdf:type        owl:Class ;
    rdfs:subClassOf semts:DataKnowledge ;
    rdfs:label      "Segment Property"@en ;
    rdfs:comment    "Generic class to specify characteristical information directly derived or generated from the time series data"@en .


###  https://w3id.org/semts/ontology#SeriesComponentGroup
semts:SeriesComponentGroup
    rdf:type        owl:Class ;
    rdfs:subClassOf semts:DataKnowledge, semts:KnowledgeGroup, [ rdf:type          owl:Restriction ;
                                                                 owl:onProperty    semts:groupKnowledge ;
                                                                 owl:allValuesFrom semts:SegmentProperty ] ;
    rdfs:label      "Series Component Group"@en ;
    rdfs:comment    "Groups extracted time series features"@en .


###  https://w3id.org/semts/ontology#SeriesComponentProperty
semts:SeriesComponentProperty
    rdf:type        owl:Class ;
    rdfs:subClassOf semts:SegmentProperty ;
    rdfs:label      "Series Component Property"@en ;
    rdfs:comment    "Characterises all properties, which describe extracted time series features"@en .


###  https://w3id.org/semts/ontology#SeriesData
semts:SeriesData
    rdf:type        owl:Class ;
    rdfs:subClassOf mls:Dataset ;
    rdfs:label      "Series Data"@en ;
    rdfs:comment    "References and defines time series metadata"@en .


###  https://w3id.org/semts/ontology#SeriesDimension
semts:SeriesDimension
    rdf:type        owl:Class ;
    rdfs:subClassOf mls:Feature ;
    rdfs:label      "Series Dimension"@en ;
    rdfs:comment    "Defines metadata of a time series dimension"@en .


###  https://w3id.org/semts/ontology#Settings
semts:Settings
    rdf:type        owl:Class ;
    rdfs:subClassOf semts:KnowledgeGroup, semts:ScenarioKnowledge, [ rdf:type          owl:Restriction ;
                                                                     owl:onProperty    semts:groupKnowledge ;
                                                                     owl:allValuesFrom semts:ScenarioParameter ] ;
    rdfs:label      "Settings"@en ;
    rdfs:comment    "A particular knowledge group to define scenario parameters"@en .


###  https://w3id.org/semts/ontology#StructuralComponentConcept
semts:StructuralComponentConcept
    rdf:type        owl:Class ;
    rdfs:subClassOf skos:Concept ;
    rdfs:label      "Structural Component Concept"@en ;
    rdfs:comment    "Concept to describe knowledge of type structure"@en .


###  https://w3id.org/semts/ontology#TimeIndex
semts:TimeIndex
    rdf:type        owl:Class ;
    rdfs:subClassOf time:TemporalEntity ;
    rdfs:label      "Time Index"@en ;
    rdfs:comment    "Defines the index of a time series segment"@en .


###  https://w3id.org/semts/ontology#TrendComponentConcept
semts:TrendComponentConcept
    rdf:type        owl:Class ;
    rdfs:subClassOf skos:Concept ;
    rdfs:label      "Trend Component Concept"@en ;
    rdfs:comment    "Concept to describe knowledge of type trend"@en .
