@prefix : <https://w3id.org/semts/vocabulary/scenario-knowledge#> .
@prefix owl: <http://www.w3.org/2002/07/owl#> .
@prefix rdf: <http://www.w3.org/1999/02/22-rdf-syntax-ns#> .
@prefix rdfs: <http://www.w3.org/2000/01/rdf-schema#> .
@prefix skos: <http://www.w3.org/2004/02/skos/core#> .
@prefix semts: <https://w3id.org/semts/ontology#> .
@base <https://w3id.org/semts/vocabulary/scenario-knowledge#> .

#################################################################
#    Properties
#################################################################

###  http://www.w3.org/2004/02/skos/core#definition
skos:definition rdf:type owl:AnnotationProperty .

###  http://www.w3.org/2004/02/skos/core#member
skos:member rdf:type owl:AnnotationProperty .

###  http://www.w3.org/2004/02/skos/core#prefLabel
skos:prefLabel rdf:type owl:AnnotationProperty .

###  http://www.w3.org/2004/02/skos/core#broader
skos:broader rdf:type owl:ObjectProperty .

###  http://www.w3.org/2004/02/skos/core#narrower
skos:narrower rdf:type owl:ObjectProperty .

#################################################################
#    Classes
#################################################################

###  http://www.w3.org/2004/02/skos/core#Collection
skos:Collection rdf:type owl:Class .

###  http://www.w3.org/2004/02/skos/core#Concept
skos:Concept rdf:type owl:Class .

###  https://w3id.org/semts/ontology#KnowledgeConcept
semts:KnowledgeConcept rdf:type owl:Class ; 
  rdfs:subClassOf skos:Concept .

#################################################################
#    Scenario Knowledge Concepts
#################################################################

###  https://w3id.org/semts/vocabulary/scenario-knowledge#ScenarioKnowledge
:ScenarioKnowledge rdf:type owl:NamedIndividual, semts:KnowledgeConcept ;
  skos:prefLabel "Scenario Knowledge" ;
  skos:definition "Scenario Knowledge encompasses structured information and insights relevant to understanding and analyzing specific situations in time series data." .

###  https://w3id.org/semts/vocabulary/scenario-knowledge#Annotation
:Annotation rdf:type owl:NamedIndividual, semts:KnowledgeConcept ;
  skos:prefLabel "Annotation" ;
  skos:broader :ScenarioKnowledge ;
  skos:definition "Annotations are notes or labels added to time series data to provide additional context or information for better understanding." .

###  https://w3id.org/semts/vocabulary/scenario-knowledge#Note
:Note rdf:type owl:NamedIndividual, semts:KnowledgeConcept ;
  skos:prefLabel "Note" ;
  skos:broader :ScenarioKnowledge ;
  skos:definition "Notes are brief pieces of information that are added to time series data to highlight important aspects or observations." .

###  https://w3id.org/semts/vocabulary/scenario-knowledge#ContextualInformation
:ContextualInformation rdf:type owl:NamedIndividual, semts:KnowledgeConcept ;
  skos:prefLabel "Contextual Information" ;
  skos:broader :Note ;
  skos:definition "Contextual Information provides background or situational details that enhance the understanding of time series data." .

###  https://w3id.org/semts/vocabulary/scenario-knowledge#Fact
:Fact rdf:type owl:NamedIndividual, semts:KnowledgeConcept ;
  skos:prefLabel "Fact" ;
  skos:broader :ContextualInformation ;
  skos:definition "Evaluated statement that holds true and equals ground truth information." .

###  https://w3id.org/semts/vocabulary/scenario-knowledge#InformalComment
:InformalComment rdf:type owl:NamedIndividual, semts:KnowledgeConcept ;
  skos:prefLabel "Informal Comment" ;
  skos:broader :Note ;
  skos:definition "An informal note which can literally be any arbitrary message that is not covered by a predefined category." .

###  https://w3id.org/semts/vocabulary/scenario-knowledge#Rule
:Rule rdf:type owl:NamedIndividual, semts:KnowledgeConcept ;
  skos:prefLabel "Rule" ;
  skos:broader :ContextualInformation ;
  skos:definition "Information which can be regarded a guideline, restriction or instruction." .

###  https://w3id.org/semts/vocabulary/scenario-knowledge#Observation
:Observation rdf:type owl:NamedIndividual, semts:KnowledgeConcept ;
  skos:prefLabel "Observation" ;
  skos:broader :Note ;
  skos:definition "Observations are specific insights derived from time series data that are influenced by the surrounding context." .

###  https://w3id.org/semts/vocabulary/scenario-knowledge#Assumption
:Assumption rdf:type owl:NamedIndividual, semts:KnowledgeConcept ;
  skos:prefLabel "Assumption" ;
  skos:broader :ContextualInformation ;
  skos:definition "Assumptions are hypotheses or premises considered within the context of analyzing time series data." .

###  https://w3id.org/semts/vocabulary/scenario-knowledge#ScenarioParameter
:ScenarioParameter rdf:type owl:NamedIndividual, semts:KnowledgeConcept ;
  skos:prefLabel "Scenario Parameter" ;
  skos:broader :ScenarioKnowledge ;
  skos:definition "Scenario Parameters are variables related to specific scenarios." .

###  https://w3id.org/semts/vocabulary/scenario-knowledge#MathExpression
:MathExpression rdf:type owl:NamedIndividual, semts:KnowledgeConcept ;
  skos:prefLabel "Math Expression" ;
  skos:broader :ScenarioKnowledge ;
  skos:definition "Math Expressions are mathematical formulas or equations used to model or analyze time series data." .

###  https://w3id.org/semts/vocabulary/scenario-knowledge#BooleanEquation
:BooleanEquation rdf:type owl:NamedIndividual, semts:KnowledgeConcept ;
  skos:prefLabel "Boolean Equation" ;
  skos:broader :MathExpression ;
  skos:definition "Boolean Equations involve logical operators and logical expressions." .

###  https://w3id.org/semts/vocabulary/scenario-knowledge#Condition
:Condition rdf:type owl:NamedIndividual, semts:KnowledgeConcept ;
  skos:prefLabel "Condition" ;
  skos:broader :BooleanEquation ;
  skos:definition "Boolean expressions used to evaluate conditions within time series data." .

###  https://w3id.org/semts/vocabulary/scenario-knowledge#AlgebraicEquation
:AlgebraicEquation rdf:type owl:NamedIndividual, semts:KnowledgeConcept ;
  skos:prefLabel "Algebraic Equation" ;
  skos:broader :MathExpression ;
  skos:definition "Algebraic Equations are mathematical statements consisting of algebraic expressions used in the analysis of time series data." .

###  https://w3id.org/semts/vocabulary/scenario-knowledge#DifferentialEquation
:DifferentialEquation rdf:type owl:NamedIndividual, semts:KnowledgeConcept ;
  skos:prefLabel "Differential Equation" ;
  skos:broader :MathExpression ;
  skos:definition "Differential Equations involve derivatives and are used to model dynamic changes and trends in time series data." .

###  https://w3id.org/semts/vocabulary/scenario-knowledge#PolynomialEquation
:PolynomialEquation rdf:type owl:NamedIndividual, semts:KnowledgeConcept ;
  skos:prefLabel "Polynomial Equation" ;
  skos:broader :MathExpression ;
  skos:definition "Polynomial Equations consist of terms raised to powers, representing relationships and patterns within time series data." .

###  https://w3id.org/semts/vocabulary/scenario-knowledge#ExponentialEquation
:ExponentialEquation rdf:type owl:NamedIndividual, semts:KnowledgeConcept ;
  skos:prefLabel "Exponential Equation" ;
  skos:broader :MathExpression ;
  skos:definition "Exponential Equations model growth or decay processes in time series data using exponential functions." .

###  https://w3id.org/semts/vocabulary/scenario-knowledge#LogarithmicEquation
:LogarithmicEquation rdf:type owl:NamedIndividual, semts:KnowledgeConcept ;
  skos:prefLabel "Logarithmic Equation" ;
  skos:broader :MathExpression ;
  skos:definition "Logarithmic Equations involve logarithms and are used to model multiplicative relationships in time series data." .

###  https://w3id.org/semts/vocabulary/scenario-knowledge#TrigonometricEquation
:TrigonometricEquation rdf:type owl:NamedIndividual, semts:KnowledgeConcept ;
  skos:prefLabel "Trigonometric Equation" ;
  skos:broader :MathExpression ;
  skos:definition "Trigonometric Equations use trigonometric functions to represent periodic patterns and cycles in time series data." .

###  https://w3id.org/semts/vocabulary/scenario-knowledge#IntegralEquation
:IntegralEquation rdf:type owl:NamedIndividual, semts:KnowledgeConcept ;
  skos:prefLabel "Integral Equation" ;
  skos:broader :MathExpression ;
  skos:definition "Integral Equations involve integrals and are used to analyze cumulative effects and total values in time series data." .

###  https://w3id.org/semts/vocabulary/scenario-knowledge#Label
:Label rdf:type owl:NamedIndividual, semts:KnowledgeConcept ;
  skos:prefLabel "Label" ;
  skos:broader :Annotation ;
  skos:definition "Labels are identifiers or markers added to time series data to categorize or highlight specific elements or features." .

###  https://w3id.org/semts/vocabulary/scenario-knowledge#Keyword
:Keyword rdf:type owl:NamedIndividual, semts:KnowledgeConcept ;
  skos:prefLabel "Keyword" ;
  skos:broader :Annotation ;
  skos:definition "Tags that are used for categorization, organization and indexing." .

###  https://w3id.org/semts/vocabulary/scenario-knowledge#CategorizedEvent
:CategorizedEvent rdf:type owl:NamedIndividual, semts:KnowledgeConcept ;
  skos:prefLabel "Categorized Event" ;
  skos:broader :Annotation ;
  skos:definition "An event that is predefined and not an unexpected observation." .

###  https://w3id.org/semts/vocabulary/scenario-knowledge#Action
:Action rdf:type owl:NamedIndividual, semts:KnowledgeConcept ;
  skos:prefLabel "Action" ;
  skos:broader :CategorizedEvent ;
  skos:definition "An action that equals a predefined event. Commonly performed to change or correct a certain process behavior." .

###  https://w3id.org/semts/vocabulary/scenario-knowledge#UncategorizedEvent
:UncategorizedEvent rdf:type owl:NamedIndividual, semts:KnowledgeConcept ;
  skos:prefLabel "Uncategorized Event" ;
  skos:broader :Observation ;
  skos:definition "An event that is not predefined and thus an unexpected observation or action." .

#################################################################
#    Scenario Knowledge Collections
#################################################################

### https://w3id.org/semts/vocabulary/data-knowledge#Settings
:Setting rdf:type owl:NamedIndividual, skos:Collection, semts:KnowledgeConcept ;
    skos:prefLabel "Setting"@en ;
    skos:definition "A collection of scenario parameters which together represent a setting."@en ;
    skos:member :ScenarioParameter .
